end of day 15/12/18

michael_formal/not4afp/Drinks_Machine_Change.thy
@@ -2,6 +2,8 @@ theory Drinks_Machine_Change
   imports "../examples/Drinks_Machine"
 begin
 
+declare One_nat_def[simp del]
+
 definition vend :: "transition" where
 "vend \<equiv> \<lparr>
         Label = ''vend'',
@@ -11,113 +13,87 @@ definition vend :: "transition" where
         Updates = [(R 1, (V (R 1))), (R 2, (V (R 2)))]
       \<rparr>"
 
-definition drinks :: "Drinks_Machine.statename efsm" where
-"drinks \<equiv> \<lparr> 
-          s0 = q1,
-          T = \<lambda> (a,b) .
-                   if (a,b) = (q1,q2) then {select} (* If we want to go from state 1 to state 2 then select will do that *)
-              else if (a,b) = (q2,q2) then {coin} (* If we want to go from state 2 to state 2 then coin will do that *)
-              else if (a,b) = (q2,q3) then {vend} (* If we want to go from state 2 to state 3 then drinks will do that *)
-              else {} (* There are no other transitions *)
-         \<rparr>"
-
-lemma s0_drinks [simp]: "s0 drinks = q1"
-  by (simp add: drinks_def)
+definition drinks :: transition_matrix where
+"drinks \<equiv> {|
+             ((0,1), select), (* If we want to go from state 0 to state 1 then select will do that *)
+             ((1,1), coin),   (* If we want to go from state 1 to state 1 then coin will do that *)
+             ((1,2), vend)    (* If we want to go from state 1 to state 2 then vend will do that *)
+         |}"
 
 lemmas transitions = select_def coin_def vend_def
 
-lemma "observe_trace drinks (s0 drinks) <> [] = []"
-  by simp
+lemma "observe_trace drinks 0 <> [] = []"
+  by (simp add: observe_trace_def)
 
-lemma label_select_q2: "Label b = ''select'' \<Longrightarrow> b \<in> T drinks (q1, a) \<Longrightarrow> b = select \<and> a = q2"
-  apply (simp add: drinks_def)
-  apply (cases a)
-  by simp_all
+lemma possible_steps_0:  "length i = 1 \<Longrightarrow> possible_steps drinks 0 Map.empty (''select'') i = {|(1, select)|}"
+  apply (simp add: possible_steps_def drinks_def transitions)
+  by force
 
-lemma possible_steps_q1: "possible_steps drinks q1 Map.empty ''select'' [Str ''coke''] = {(q2, select)}"
-  apply (simp add: possible_steps_def)
-  apply safe
-       apply (simp add: label_select_q2)
-      apply (simp add: label_select_q2)
-     apply (simp add: select_def)
-    apply (simp add: drinks_def)
-   apply (simp add: select_def)
-  by (simp add: select_def)
-
-lemma "observe_trace drinks (s0 drinks) <> [(''select'', [Str ''coke''])] = [[]]"
-  by (simp add: possible_steps_q1)
-
-lemma label_coin_q2: "Label b = ''coin'' \<Longrightarrow> b \<in> T drinks (q2, a) \<Longrightarrow> b = coin \<and> a = q2"
-  apply (simp add: drinks_def)
-  apply (cases a)
-  by (simp_all add: vend_def)
-
-lemma possible_steps_q2_coin: "possible_steps drinks q2 r ''coin'' [Num n'] = {(q2, coin)}"
-    apply (simp add: possible_steps_def)
-  apply safe
-       apply (simp add: label_coin_q2)
-      apply (simp add: label_coin_q2)
-     apply (simp add: coin_def)
-    apply (simp add: drinks_def coin_def)
-   apply (simp add: coin_def)
-  by (simp add: coin_def)
-
-lemma label_vend_q3: "Label b = ''vend'' \<Longrightarrow> b \<in> T drinks (q2, a) \<Longrightarrow> b = vend \<and> a = q3"
-  apply (simp add: drinks_def)
-  apply (cases a)
-  by (simp_all add: coin_def)
-
-lemma possible_steps_q2_vend: "n \<ge> 100 \<Longrightarrow> possible_steps drinks q2 <R (Suc 0) := Str ''coke'', R 2 := Num n> ''vend'' [] = {(q3, vend)}"
-  apply (simp add: possible_steps_def)
-  apply safe
-       apply (simp add: label_vend_q3)
-      apply (simp add: label_vend_q3)
-     apply (simp add: vend_def)
-    apply (simp add: vend_def drinks_def)
-   apply (simp add: vend_def)
-  by (simp add: vend_def)
-
-lemma updates_coin_150 [simp]: "(apply_updates (Updates coin)
-          (case_vname (\<lambda>n. if n = Suc 0 then Some (Num 100) else input2state [] (Suc 0 + 1) (I n)) (\<lambda>n. if n = 2 then Some (Num 50) else <R (Suc 0) := Str ''coke''> (R n)))
-          <R (Suc 0) := Str ''coke'', R 2 := Num 50>) = <R 1 := Str ''coke'', R 2 := Num 150>"
-  apply (rule ext)
-  by (simp add: coin_def)
-
-lemma "observe_trace drinks (s0 drinks) <> [(''select'', [Str ''coke'']), (''coin'', [Num 50]), (''coin'', [Num 50]), (''vend'', [])] = [[], [Num 50], [Num 100], [Str ''coke'', Num 0]]"
-  apply (simp add: possible_steps_q1 possible_steps_q2_coin possible_steps_q2_vend)
+lemma "observe_trace drinks 0 <> [(''select'', [Str ''coke''])] = [[]]"
+  unfolding observe_trace_def observe_all_def step_def
+  apply (simp add: possible_steps_0)
   by (simp add: transitions)
 
-lemma "observe_trace drinks (s0 drinks) <> [(''select'', [Str ''coke'']), (''coin'', [Num 50]), (''coin'', [Num 100]), (''vend'', [])] = [[], [Num 50], [Num 150], [Str ''coke'', Num 50]]"
-  apply (simp add: possible_steps_q1 possible_steps_q2_coin possible_steps_q2_vend)
-  by (simp add: transitions)
+lemma possible_steps_1_coin: "possible_steps drinks 1 r ''coin'' [Num n'] = {|(1, coin)|}"
+  apply (simp add: possible_steps_def drinks_def transitions)
+  by force
 
-lemma step_invalid: "possible_steps drinks q2 d ''invalid'' [Num 50] = {}"
-  apply (simp add: possible_steps_def drinks_def)
-  by (simp add: vend_def coin_def)
+lemma possible_steps_1_vend: "n \<ge> 100 \<Longrightarrow> possible_steps drinks 1 <R 1 := Str ''coke'', R 2 := Num n> ''vend'' [] = {|(2, vend)|}"
+  apply (simp add: possible_steps_def drinks_def transitions)
+  by force
+
+lemma "observe_trace drinks 0 <> [(''select'', [Str ''coke'']), (''coin'', [Num 50]), (''coin'', [Num 50]), (''vend'', [])] = [[], [Num 50], [Num 100], [Str ''coke'', Num 0]]"
+  unfolding observe_trace_def observe_all_def step_def
+  apply (simp add: possible_steps_0 updates_select outputs_select)
+  apply (simp add: possible_steps_1_coin updates_coin)
+  apply (simp add: possible_steps_1_vend)
+  by (simp add: coin_def vend_def)
+
+lemma "observe_trace drinks 0 <> [(''select'', [Str ''coke'']), (''coin'', [Num 50]), (''coin'', [Num 100]), (''vend'', [])] = [[], [Num 50], [Num 150], [Str ''coke'', Num 50]]"
+  unfolding observe_trace_def observe_all_def step_def
+  apply (simp add: possible_steps_0 updates_select outputs_select)
+  apply (simp add: possible_steps_1_coin updates_coin)
+  apply (simp add: possible_steps_1_vend)
+  by (simp add: coin_def vend_def)
+
+lemma possible_steps_invalid: "l \<noteq> ''coin'' \<and> l \<noteq> ''vend'' \<Longrightarrow> possible_steps drinks 1 d l i = {||}"
+  apply (simp add: possible_steps_def drinks_def transitions)
+  by force
 
 (*Stop when we hit a spurious input*)
-lemma "observe_trace drinks (s0 drinks) <> [(''select'', [Str ''coke'']), (''invalid'', [Num 50])] = [[]]"
-  by (simp add: possible_steps_q1 step_invalid is_singleton_def)
+lemma "observe_trace drinks 0 <> [(''select'', [Str ''coke'']), (''invalid'', [Num 50])] = [[]]"
+  unfolding observe_trace_def observe_all_def step_def
+  apply (simp add: possible_steps_0 updates_select outputs_select)
+  by (simp add: possible_steps_invalid)
 
-lemma invalid_input: "valid drinks q2 d' [(''invalid'', [Num 50])] \<Longrightarrow> False"
-  apply (cases rule: valid.cases)
+lemma invalid_input: "\<not> EFSM.valid drinks 1 d' [(''invalid'', [Num 50])]"
+  apply safe
+  apply (rule EFSM.valid.cases)
     apply simp
    apply simp
-  apply clarify
-  by (simp add: step_invalid is_singleton_def)
+  apply (simp add: step_def)
+  using possible_steps_invalid
+  by auto
 
 lemma invalid_valid_prefix: "\<not> (valid_trace (drinks) [(''select'', [Str ''coke'']), (''invalid'', [Num 50])])"
+  unfolding valid_trace_def
   apply clarify
-  apply (cases rule: valid.cases)
+  apply (rule EFSM.valid.induct)
     apply simp
    apply simp
+   defer
+   apply simp
+  apply (rule EFSM.valid.cases)
+    apply simp
+   apply simp
+  apply (simp add: step_def)
   apply clarify
-  apply (simp add: possible_steps_q1 invalid_input)
-  using invalid_input by force
+  apply (simp add: possible_steps_0 outputs_select updates_select)
+  using invalid_input
+  by simp
 
-lemma "observe_trace drinks (s0 drinks) <> [(''select'', [Str ''coke'']), (''invalid'', [Num 50]), (''coin'', [Num 50])] = [[]]"
-  by (simp add: possible_steps_q1 step_invalid is_singleton_def)
-
-lemma "( t = []) \<Longrightarrow> (observe_trace e (s0 e) <> t = []) "
-  by(simp)
+lemma "observe_trace drinks 0 <> [(''select'', [Str ''coke'']), (''invalid'', [Num 50]), (''coin'', [Num 50])] = [[]]"
+  unfolding observe_trace_def observe_all_def step_def
+  apply (simp add: possible_steps_0 outputs_select updates_select)
+  by (simp add: possible_steps_invalid)
 end
